Surface/Examples/Boolean.lean
@@ -12,8 +12,8 @@ def benv : GlobalEnv := [
   -- .classDecl "Id" #(★, ★) [] [⟨"fd", 0, #(0), 1⟩, ⟨"bwk", 0, #(1), 0⟩] [],
 
   -- .instDecl "EqBoolI" ⟨1, #(★), 0, #(), 1, #(gt#"Bool"), gt#"Eq" • t#0⟩ [("eq", λˢ[gt#"Bool"] λˢ[gt#"Bool"] `#0)],
-  .classDecl "Ord" #(★) [("supOrd", "Eq", [0])] [] [("leq", ⟨0, #(), 0, #(), 0, #(), t#0 -:> (t#0 -:> gt#"Ordering")⟩)],
-  .classDecl "Eq" #(★) [] [] [("eq",  ⟨0, #(), 0, #(), 0, #(), t#0 -:> (t#0 -:> gt#"Bool")⟩)],
+  .classDecl "Ord" #(★) /-[("supOrd", "Eq", [0])] []-/ [("leq", ⟨0, #(), 0, #(), 0, #(), t#0 -:> (t#0 -:> gt#"Ordering")⟩)],
+  .classDecl "Eq" #(★) /-[] []-/ [("eq",  ⟨0, #(), 0, #(), 0, #(), t#0 -:> (t#0 -:> gt#"Bool")⟩)],
   .data (n := 2) "Bool" ★ #(("True", ⟨0, #(), 0, #(), 0,  #(), gt#"Bool"⟩),
                             ("False", ⟨0, #(), 0, #(), 0, #(), gt#"Bool"⟩)),
   .data (n := 3) "Ordering" ★ #( ("LT", ⟨0, #(), 0, #(), 0,  #(), gt#"Ordering"⟩)
